platform/cito/SepHints3.v
@@ -1,0 +1,21 @@
+Require Import AutoSep.
+Require Import List.
+
+Set Implicit Arguments.
+
+Definition array_to_locals ls p (_ : list string) := array ls p.
+
+Definition array_to_locals_ok (ls : list W) (vars : list string) := length vars = length ls /\ NoDup vars.
+
+Lemma array_to_locals_fwd : forall ls p vars, array_to_locals_ok ls vars -> array_to_locals ls p vars ===> Ex vs, locals vars vs 0 p * [| toArray vars vs = ls |].
+  admit.
+Qed.
+
+Definition hints_array_to_locals : TacPackage.
+  prepare array_to_locals_fwd tt.
+Defined.
+
+Lemma replace_array_to_locals : forall ls p vars, array ls p = array_to_locals ls p vars.
+  eauto.
+Qed.
+
